Developping tactics to automatically deal with heap hypotheses.

low/Invariants.v
@@ -6,6 +6,8 @@ Set Implicit Arguments.
 Require Import TLC.LibBag.
 Require Export Rinit Rfeatures Path.
 
+Open Scope list_scope. (* FIXME: How to disable some notations of LibBag? *)
+
 
 (** * Predicates to speak about the memory **)
 
@@ -13,7 +15,7 @@ Require Export Rinit Rfeatures Path.
 
 Definition bound (S : state) p := exists p_, read_SExp S p = Some p_.
 
-(** ** A pointer is associated a given type **)
+(** ** Typed pointers **)
 
 Definition may_have_type (S : state) p l :=
   exists p_, read_SExp S p = Some p_ /\ type p_ \in l.
@@ -37,22 +39,67 @@ Proof.
   rewrite~ BagInter_list.
 Qed.
 
+Lemma may_have_type_weaken : forall S p l1 l2,
+  may_have_type S p l1 ->
+  l1 \c l2 ->
+  may_have_type S p l2.
+Proof. introv (p_&E&M) I. exists p_. splits~. applys~ BagInIncl M I. Qed.
+
+
 (** ** List pointers **)
 
-Inductive list_type (S : state) p l_t l_car l_tag : Prop := make_list_type {
-  list_type_intro : exists p_ header car cdr tag,
+Definition list_type_step P (S : state) p l_t l_car l_tag : Prop :=
+  exists p_ header car cdr tag,
     read_SExp S p = Some p_
     /\ p_ = make_NonVector_SExpRec header (make_ListSxp_struct car cdr tag)
     /\ type p_ \in l_t
     /\ may_have_type S car l_car
-    /\ list_type S cdr l_t l_car l_tag
-    /\ may_have_type S tag l_tag
-  }.
+    /\ P S cdr l_t l_car l_tag
+    /\ may_have_type S tag l_tag.
+
+Inductive list_type (S : state) : SEXP -> list SExpType -> list SExpType -> list SExpType -> Prop :=
+  | list_type_nil : forall p l_t l_car l_tag,
+    may_have_type S p ([NilSxp]) ->
+    list_type S p l_t l_car l_tag
+  | list_type_cons : forall p l_t l_car l_tag,
+    list_type_step list_type S p l_t l_car l_tag ->
+    list_type S p l_t l_car l_tag
+  .
+
+Fixpoint list_type_ind' S
+    (P : SEXP -> list SExpType -> list SExpType -> list SExpType -> Prop)
+    (f_nil : forall p l_t l_car l_tag,
+       may_have_type S p ([NilSxp]) ->
+       P p l_t l_car l_tag)
+    (f_cons : forall p l_t l_car l_tag p_ header car cdr tag,
+       read_SExp S p = Some p_ ->
+       p_ = make_NonVector_SExpRec header (make_ListSxp_struct car cdr tag) ->
+       type p_ \in l_t ->
+       may_have_type S car l_car ->
+       list_type S cdr l_t l_car l_tag ->
+       may_have_type S tag l_tag ->
+       P cdr l_t l_car l_tag ->
+       P p l_t l_car l_tag)
+    p l_t l_car l_tag (HL : list_type S p l_t l_car l_tag) : P p l_t l_car l_tag.
+  refine (
+    match HL in list_type _ p l_t l_car l_tag return P p l_t l_car l_tag with
+    | @list_type_nil _ p l_t l_car l_tag N =>
+      f_nil p l_t l_car l_tag N
+    | @list_type_cons _ p l_t l_car l_tag N => _
+    end).
+  destruct N as (p_&h&car&cdr&tag&E&M&H&A&L&T).
+  refine (f_cons p l_t l_car l_tag _ _ _ _ _ E M H A L T _).
+  applys~ list_type_ind' f_nil f_cons.
+Defined.
 
 Lemma list_type_may_have_type : forall S p l_t l_car l_tag,
   list_type S p l_t l_car l_tag ->
-  may_have_type S p l_t.
-Proof. introv [(p_&?&?&?&?&?&?&?&?&?&?)]. exists* p_. Qed.
+  may_have_type S p (l_t \u [NilSxp]).
+Proof.
+  introv I. destruct~ I as [? ? ? ? I|? ? ? ? (p_&h&car&cdr&tag&E&M&H&A&L&T)].
+  - applys may_have_type_weaken I. apply~ BagUnionIncl_right.
+  - exists p_. splits~. applys~ BagInIncl H. apply~ BagUnionIncl_left.
+Qed.
 
 Lemma list_type_merge : forall S p l1_t l2_t l1_car l2_car l1_tag l2_tag,
   list_type S p l1_t l1_car l1_tag ->
@@ -60,15 +107,35 @@ Lemma list_type_merge : forall S p l1_t l2_t l1_car l2_car l1_tag l2_tag,
   list_type S p (l1_t \n l2_t) (l1_car \n l2_car) (l1_tag \n l2_tag).
 Proof.
   introv T1 T2. gen l2_t l2_car l2_tag.
-  induction T1 as [(p1_&h1&car1&cdr1&tag1&E1&M1&H1&A1&L1&T1)].
-  introv [(p2_&h2&car2&cdr2&tag2&E2&M2&H2&A2&L2&T2)].
-  constructors. exists p1_ h1 car1 cdr1 tag1.
-  rewrite E1 in E2. inversion E2 as [E3]. rewrite E3 in *.
-  rewrite M2 in M1. inverts M1. splits~.
-  - rewrite~ BagInter_list.
-  - apply~ may_have_type_merge.
-  - 
-  - apply~ may_have_type_merge.
+  induction T1 as [? ? ? ? I1|? ? ? ? p1_ h1 car1 cdr1 tag1 E1 M1 H1 A1 L1 T1 IH]
+    using list_type_ind'; introv T.
+  - apply~ list_type_nil.
+  - inverts T as T.
+    + apply~ list_type_nil.
+    + inverts T as (h2&car2&cdr2&tag2&E2&M2&H2&A2&L2&T2).
+      rewrite E2 in E1. inversion E1 as [E1']. rewrite E1' in *.
+      rewrite M1 in M2. inverts M2.
+      apply list_type_cons. exists p1_ h2 car2 cdr2 tag2. splits~.
+      * apply BagInter_list. splits~.
+      * applys~ may_have_type_merge A1 A2.
+      * applys~ may_have_type_merge T1 T2.
+Qed.
+
+Lemma list_type_weaken : forall S p l1_t l2_t l1_car l2_car l1_tag l2_tag,
+  l1_t \c l2_t ->
+  l1_car \c l2_car ->
+  l1_tag \c l2_tag ->
+  list_type S p l1_t l1_car l1_tag ->
+  list_type S p l2_t l2_car l2_tag.
+Proof.
+  introv I1 I2 I3 T. gen l2_t l2_car l2_tag.
+  induction T as [? ? ? ? I1|? ? ? ? p_ h car cdr tag E M H A L T IH]
+    using list_type_ind'; introv Incl1 Incl2 Incl3.
+  - apply~ list_type_nil.
+  - apply list_type_cons. exists p_ h car cdr tag. splits~.
+    + applys~ BagInIncl H Incl1.
+    + applys~ may_have_type_weaken A Incl2.
+    + applys~ may_have_type_weaken T Incl3.
 Qed.
 
 
@@ -81,35 +148,35 @@ Record safe_SExpRec S (e_ : SExpRec) := make_safe_SExpRec {
       type e_ = NilSxp ->
       exists header car cdr tag,
         e_ = make_NonVector_SExpRec header (make_ListSxp_struct car cdr tag)
-        /\ may_have_type S car [NilSxp]
-        /\ may_have_type S cdr [NilSxp]
-        /\ may_have_type S tag [NilSxp] ;
+        /\ may_have_type S car ([NilSxp])
+        /\ may_have_type S cdr ([NilSxp])
+        /\ may_have_type S tag ([NilSxp]) ;
     SExpType_corresponds_to_data_SymSxp :
       type e_ = SymSxp ->
       exists header pname value internal,
         e_ = make_NonVector_SExpRec header (make_SymSxp_struct pname value internal)
-        /\ may_have_type S pname [CharSxp]
-        (*/\ may_have_type S value [(*TODO*)]
-        /\ may_have_type S internal [(*TODO*)]*) ;
+        /\ may_have_type S pname ([CharSxp])
+        (*/\ may_have_type S value ([(*TODO*)])
+        /\ may_have_type S internal ([(*TODO*)])*) ;
     SExpType_corresponds_to_data_ListSxp :
       type e_ = ListSxp ->
       exists header car cdr tag,
         e_ = make_NonVector_SExpRec header (make_ListSxp_struct car cdr tag)
-        /\ may_have_type S cdr [ListSxp]
-        /\ may_have_type S tag [NilSxp ; CharSxp] ;
+        /\ may_have_type S cdr ([ListSxp])
+        /\ may_have_type S tag ([NilSxp ; CharSxp]) ;
     SExpType_corresponds_to_data_CloSxp :
       type e_ = CloSxp ->
       exists header formals body env,
         e_ = make_NonVector_SExpRec header (make_CloSxp_struct formals body env)
-        /\ may_have_type S formals [NilSxp ; ListSxp]
-        (*/\ may_have_type S body [(*TODO*)]*)
-        /\ may_have_type S env [EnvSxp] ;
+        /\ may_have_type S formals ([NilSxp ; ListSxp])
+        (*/\ may_have_type S body ([(*TODO*)])*)
+        /\ may_have_type S env ([EnvSxp]) ;
     SExpType_corresponds_to_data_EnvSxp :
       type e_ = EnvSxp ->
       exists header frame enclos,
         e_ = make_NonVector_SExpRec header (make_EnvSxp_struct frame enclos)
-        /\ may_have_type S frame [NilSxp ; ListSxp]
-        /\ may_have_type S enclos [EnvSxp] ;
+        /\ may_have_type S frame ([NilSxp ; ListSxp])
+        /\ may_have_type S enclos ([EnvSxp]) ;
     SExpType_corresponds_to_data_SpecialSxp :
       type e_ = SpecialSxp ->
       exists header offset,
@@ -150,14 +217,14 @@ Record safe_SExpRec S (e_ : SExpRec) := make_safe_SExpRec {
                (make_VecSxp_struct (ArrayList.length array) array))
         /\ forall a,
           Mem a (ArrayList.to_list array) ->
-          may_have_type S a [CharSxp] ;
+          may_have_type S a ([CharSxp]) ;
     SExpType_corresponds_to_data_DotSxp :
       type e_ = DotSxp ->
       exists header car cdr tag,
         e_ = make_NonVector_SExpRec header (make_ListSxp_struct car cdr tag)
-        (*/\ may_have_type S car [(*TODO*)]*)
-        /\ may_have_type S cdr [ListSxp]
-        /\ may_have_type S tag [NilSxp] ;
+        (*/\ may_have_type S car ([(*TODO*)])*)
+        /\ may_have_type S cdr ([ListSxp])
+        /\ may_have_type S tag ([NilSxp]) ;
     SExpType_not_AnySxp :
       type e_ <> AnySxp ;
     SExpType_corresponds_to_data_VecSxp :
@@ -167,7 +234,7 @@ Record safe_SExpRec S (e_ : SExpRec) := make_safe_SExpRec {
                (make_VecSxp_struct (ArrayList.length array) array))
         (*/\ forall a,
           Mem a (ArrayList.to_list array) ->
-          may_have_type S a [(*TODO*)]*) ;
+          may_have_type S a ([(*TODO*)])*) ;
     SExpType_corresponds_to_data_ExprSxp :
       type e_ = ExprSxp ->
       exists header array,
@@ -175,7 +242,7 @@ Record safe_SExpRec S (e_ : SExpRec) := make_safe_SExpRec {
                (make_VecSxp_struct (ArrayList.length array) array))
         (*/\ forall a,
           Mem a (ArrayList.to_list array) ->
-          may_have_type S a [(*TODO*)]*) ;
+          may_have_type S a ([(*TODO*)])*) ;
     (** The following four types have not been implemented. **)
     SExpType_corresponds_to_data_BcodeSxp :
       type e_ = BcodeSxp -> True ;
@@ -225,6 +292,8 @@ Record safe_state S := make_safe_state {
 
 (** ** Simplifying tactics **)
 
+(** *** Simplifying lists **)
+
 Ltac compute_is_in x l :=
   match l with
   | nil => constr:(false)
@@ -262,6 +331,26 @@ Ltac simpl_list_inter :=
     let l := compute_list_inter l1 l2 in
     asserts_rewrite (l1 \n l2 = l) in H; [solve_eq|]
   end.
+
+
+(** *** Simplifying the context **)
+
+Ltac simplify_context :=
+  match goal with
+  | H1 : may_have_type ?S1 ?p1 ?l1,
+    H2 : may_have_type ?S2 ?p2 ?l2 |- _ =>
+    let H3 := fresh H1 H2 in
+    lets H3: may_have_type_merge (rm H1) (rm H2);
+    rename H3 into H1
+  | H1 : list_type ?S1 ?p1 ?l1_t ?l1_car ?l1_tag,
+    H2 : list_type ?S2 ?p2 ?l2_t ?l2_car ?l2_tag |- _ =>
+    let H3 := fresh H1 H2 in
+    lets H3: list_type_merge (rm H1) (rm H2);
+    rename H3 into H1
+  end; simpl_list_inter.
+
+
+
 
 (* TODO *)
 
